theories/iris/logrel/instr/typing/loop.v
@@ -51,7 +51,7 @@ Section loop.
     iApply (cwp_loop' with "[$] [$] [Hvs Hos Hframe Hrt]"); first done.
     - rewrite <- Hlen_ts1. rewrite Hlen_vs. by apply has_values_length.
     - instantiate (1 := fun fr' vs' =>
-        (⌜frame_rel lmask fr fr'⌝ ∗ frame_interp rti sr se L (wl ++ wl2 ++ wlf) fr' ∗
+        (⌜frame_rel lmask fr fr'⌝ ∗ frame_interp rti sr se F.(fc_params) F.(typing.fc_locals) L (wl ++ wl2 ++ wlf) fr' ∗
            (∃ os', values_interp rti sr se τs1 os' ∗ atoms_interp os' vs') ∗
            (∃ θ', rt_token rti sr θ'))%I).
       by iFrame.
@@ -61,7 +61,7 @@ Section loop.
       + done.
       + iPureIntro. apply has_values_to_consts.
       + by destruct Hrel as [_ ->].
-      + iApply labels_interp_cons.
+      + iSimpl. iApply labels_interp_cons.
         1, 2, 3: done.
         * iIntros "!> %fr'' %vs'' (%Hfrel & Hframe & (%os'' & Hos & Hvs) & [%θ'' Hrt])".
           iFrame.
